backend/StackingSingleStack.v
@@ -1,0 +1,46 @@
+(* *********************************************************************)
+(*                                                                     *)
+(*              The Compcert verified compiler                         *)
+(*                                                                     *)
+(*          Xavier Leroy, INRIA Paris-Rocquencourt                     *)
+(*                                                                     *)
+(*  Copyright Institut National de Recherche en Informatique et en     *)
+(*  Automatique.  All rights reserved.  This file is distributed       *)
+(*  under the terms of the INRIA Non-Commercial License Agreement.     *)
+(*                                                                     *)
+(* *********************************************************************)
+
+(** Layout of activation records; translation from Linear to Mach. *)
+
+Require Import Coqlib Errors.
+Require Import Integers AST.
+Require Import Op Locations Linear MachSingleStack.
+Require Import Bounds Conventions Stacklayout Lineartyping.
+Require Export Stacking.
+
+Local Open Scope string_scope.
+
+(** PW: We align the size of the frame to 8 so that alignment properties that
+  held in the multiple stack blocks framework, still hold now. More precisely,
+  we want that [shift_offset spofs (align ofs al) = align (shift_offset spofs
+  ofs) al], where [al] is 4 or 8. *)
+
+Definition transf_function (f: Linear.function) : res Mach.function :=
+  let fe := make_env (function_bounds f) in
+  if negb (wt_function f) then
+    Error (msg "Ill-formed Linear code")
+  else if zlt Ptrofs.max_unsigned fe.(fe_size) then
+    Error (msg "Too many spilled variables, stack size exceeded")
+  else
+    OK (Mach.mkfunction
+         f.(Linear.fn_sig)
+         (transl_body f fe)
+         (align (fe_size fe) 8)
+         (Ptrofs.repr fe.(fe_ofs_link))
+         (Ptrofs.repr fe.(fe_ofs_retaddr))).
+
+Definition transf_fundef (f: Linear.fundef) : res Mach.fundef :=
+  AST.transf_partial_fundef transf_function f.
+
+Definition transf_program (p: Linear.program) : res Mach.program :=
+  transform_partial_program transf_fundef p.
